# Composite Functions

#### ii)$ff(0.5)$

$$
\begin{aligned}
ff(0.5) &= f(\color{red}f\color{text}(0.5))\\
        &= \color{red}f\color{text}(3(0.5)+1)\\
        &= 3(\color{red}3(0.5)+1\color{text})+1\\
        &= 3(2.5)+1\\
        &= ...
\end{aligned}
$$

### b) Function inverse $f^{-1}(x)$
$$
y=f(x) \leftarrow \text{use }y\text{ notation instead of }f(x)\\
\text{swap places with }\color{red}x\color{text}\text{ and } \color{yellow}y\color{text}\\
\color{yellow}y\color{text}=3\color{red}x\color{text}+1 \iff \color{red}x\color{text}=3\color{yellow}y\color{text}+1\\
\text{in the new equation }(x=3y+1)\text{, isolate }y\\
\begin{aligned}
x &=3y+1\\
x-1 &= 3y\\
3y &= x-1\\
y &= {x-1\over{3}}\\
f^{-1}(x) &= {x-1\over{3}}
\end{aligned}
$$

### c) fg(x)

![stephen_hw1](/figs/stephen_hw1.jpg)

## 1)

$f(x)=3x+1$
$g(x)=(x+2)^2$
***
### a)
#### i)
$$
\begin{aligned}
gf(2) &= g(\color{red}f\color{text}(2))\\
      &= \color{red}g\color{text}(3(2)+2)\\
      &= (\color{red}3(2)\color{text}+2)^2\\
      &= (6\color{red}+\color{text}2)^2\\
      &= (8)\color{red}^2\color{black}\\
      &= 64
\end{aligned}
$$
